fibo32, calling an F* lemma in a Pulse term just works, since Core converts lemmas to a squashed result

pulse/share/steel/examples/pulse/Fibonacci.fst
@@ -12,7 +12,49 @@ let rec fib (n:nat) : nat =
   if n <= 1 then 1
   else fib (n - 1) + fib (n - 2)
 
-#push-options "--using_facts_from 'Prims FStar.Pervasives FStar.Ghost Fibonacci'" //" -FStar.Tactics -FStar.Reflection -Pulse +Pulse.Steel.Wrapper -Pulse.Steel.Wrapper.Typing'"
+let rec fib_mono (n:nat) (m:nat { m <= n})
+  : Lemma
+    (ensures fib m <= fib n)
+  = if n = m then ()
+    else fib_mono (n - 1) m
+
+#push-options "--using_facts_from 'Prims FStar.Pervasives FStar.Ghost FStar.UInt FStar.UInt32 Fibonacci'"
+
+```pulse
+fn fibo32 (k:(n:U32.t { 0 < U32.v n  /\ fib (U32.v n) < pow2 32 }))
+  requires emp
+  returns r:U32.t
+  ensures pure (U32.v r == fib (U32.v k))
+{
+  let mut i = 1ul;
+  let mut j = 1ul;
+  let mut ctr = 1ul;
+  while (let vctr = !ctr; U32.(vctr <^ k))
+  invariant b . exists vi vj vctr. (
+     pts_to i full_perm vi `star`
+     pts_to j full_perm vj `star`
+     pts_to ctr full_perm vctr `star`     
+     pure (1 <= U32.v vctr /\
+           U32.v vctr <= U32.v k /\
+           fib (U32.v vctr - 1) == U32.v vi/\
+           fib (U32.v vctr) == U32.v vj /\
+           b == U32.(vctr <^ k))
+  )
+  {
+     let vc = !ctr;
+     let vi = !i;
+     let vj = !j;
+     ctr := U32.(vc +^ 1ul);
+     i := vj;
+     fib_mono (U32.v k) (U32.v vc + 1);
+     j := U32.(vi +^ vj);
+     ()
+  };
+  let r = !j;
+  r
+}
+```
+
 
 ```pulse
 fn fibo (n:pos)
